theories/Undefined.v
@@ -1,0 +1,76 @@
+Require Import FreeSpec.Interface.
+Require Import FreeSpec.Program.
+Require Import FreeSpec.Compose.
+Require Import FreeSpec.Control.
+Require Import FreeSpec.Control.Classes.
+
+(** * The Shameful [Undefined] Interface
+
+    Using the [Undefined] interface, you can pledge guilty of having
+    undefined behaviour in your formal specification.
+
+    ** Definition
+
+    *)
+
+Inductive Undefined
+  : Interface :=
+| undefined {A: Type}
+  : Undefined A.
+
+(** ** Why using an Interface?
+
+    We use an Interface to deal with Undefined Behaviour for at least
+    two reasons:
+
+      * It makes obvious that a given Interpreter uses the undefined
+        primitive
+      * It is easier to write a contract to check if [undefined] is
+        called
+
+    * [UndefMonad] Typeclass
+
+    The UndefMonad is here to provide an easier way to work with
+    undefined behaviour. Indeed, this library provides the required
+    typeclass instances so that if the [Undefined] Interface is used,
+    the [undef] primitive is available on the top of the monad stack
+    (that is, after the composition of the Interfaces and the use of a
+    State Monad).
+ *)
+
+Class UndefMonad
+      (m: Type -> Type)
+  := { undef_is_monad :> Monad m
+     ; undef {A: Type}
+       : m A
+     }.
+
+Instance undefmonad_Trans
+         (t: forall (m: Type -> Type) `{Monad m}, Type -> Type)
+        `{MonadTrans t}
+         (m: Type -> Type)
+        `{UndefMonad m}
+  : UndefMonad (t m) :=
+  { undef := fun {a: Type} => lift (undef (A:=a))
+  }.
+
+Instance undefprogram_UndefMonad
+  : UndefMonad (Program Undefined) :=
+  { undef := fun {a: Type} => instr (undefined (A:=a))
+  }.
+
+Local Open Scope free_scope.
+
+Instance rightprogram_UndefMonad
+         {I I': Interface}
+        `{UndefMonad (Program I)}
+  : UndefMonad (Program (I <+> I')) :=
+  { undef := fun {a: Type} => liftl undef
+  }.
+
+Instance leftprogram_UndefMonad
+         {I I': Interface}
+        `{UndefMonad (Program I')}
+  : UndefMonad (Program (I <+> I')) :=
+  { undef := fun {a: Type} => liftr undef
+  }.
